Equiv/SimF.v
@@ -1,0 +1,209 @@
+Require Import List paco2.
+Require Export Util Var Val Exp MoreExp Env Map CSet AutoIndTac IL AllInRel Sawtooth.
+Require Export Sim SimTactics IL InRel.
+
+Set Implicit Arguments.
+Unset Printing Records.
+
+(* A proof relation is parameterized by analysis information A *)
+Class ProofRelation (A:Type) := {
+    (* Relates parameter lists according to analysis information *)
+    ParamRel : A -> list var -> list var -> Prop;
+    (* Relates argument lists according to analysis information
+       and closure environments *)
+    ArgRel : A -> list val -> list val -> Prop;
+    (* Relates blocks according to analysis information *)
+    BlockRel : A -> F.block -> F.block -> Prop;
+    (* Relates environments according to analysis information *)
+    IndexRel : 〔A〕 -> nat -> nat -> Prop;
+    Image : 〔A〕 -> nat;
+    ArgLengthMatchI : forall a Z Z' VL VL',
+        ParamRel a Z Z' -> ArgRel a VL VL' -> length Z = length VL /\ length Z' = length VL';
+    IndexRelDrop : forall AL' AL n n', IndexRel (AL' ++ AL) n n' ->
+                                  n >= length AL'
+                                  -> IndexRel AL (n - length AL') (n' - Image AL')
+(*    IndexRelApp : forall AL AL' n n', IndexRelI AL n n' -> IndexRelI (AL' ++ AL) (❬AL'❭ + n) n' *)
+}.
+
+Definition frel := rel3 simtype (fun _ : simtype => F.state)
+                       (fun (_ : simtype) (_ : F.state) => F.state).
+
+Definition indexwise_r t (r:frel) A (PR:ProofRelation A) AL' E E' F F' AL L L' :=
+  forall n n' Z s Z' s' a,
+    IndexRel (AL' ++ AL) n n'
+    -> get F n (Z,s)
+    -> get F' n' (Z',s')
+    -> get AL' n a
+    -> forall VL VL',
+        ArgRel a VL VL'
+        -> r t (mapi (F.mkBlock E) F ++ L, E[Z <-- List.map Some VL], s)
+            (mapi (F.mkBlock E') F' ++ L', E'[Z' <-- List.map Some VL'], s').
+
+Lemma indexwise_r_mon t (r r':frel) A (PR:ProofRelation A) AL' E E' F F' AL L L'
+  : indexwise_r t r PR AL' E E' F F' AL L L'
+    -> (forall t x y, r t x y -> r' t x y)
+    -> indexwise_r t r' PR AL' E E' F F' AL L L'.
+Proof.
+  intros Idx LE; hnf; intros; eauto.
+Qed.
+
+Definition simLabenv t (r:frel)
+           {A} (PR:ProofRelation A) (AL:list A) L L' :=
+  (length AL = length L /\ sawtooth L' /\ sawtooth L) /\
+  forall f f' a Z s n Z' s' n' V V',
+    IndexRel AL f f'
+    -> get AL f a
+    -> get L f (F.blockI V Z s n)
+    -> get L' f' (F.blockI V' Z' s' n')
+    -> (ParamRel a Z Z' /\ BlockRel a (F.blockI V Z s n) (F.blockI V' Z' s' n'))
+      /\ (forall E E' Yv Y'v Y Y',
+            ArgRel a Yv Y'v
+            -> omap (exp_eval E) Y = Some Yv
+            -> omap (exp_eval E') Y' = Some Y'v
+            -> sim'r r t (drop (f  - n) L, E, stmtApp (LabI n) Y)
+                    (drop (f'  - n') L', E', stmtApp (LabI n') Y')).
+
+Lemma simILabenv_mon t (r r':frel) A (PR:ProofRelation A) AL L L'
+  : simLabenv t r PR AL L L'
+    -> (forall t x y, r t x y -> r' t x y)
+    -> simLabenv t r' PR AL L L'.
+Proof.
+  intros [[? ?] SIM] LE; hnf; intros; split; eauto.
+  intros. edestruct SIM as [[? ?] SIM']; eauto.
+  split; eauto. intros.
+  eapply paco3_mon. eapply SIM; eauto. eauto.
+Qed.
+
+Definition indexwise_proofrel A (PR:ProofRelation A) E E' (F F':〔params * stmt〕) AL' AL :=
+  forall n n' Z s Z' s' a,
+    IndexRel (AL' ++ AL) n n'
+    -> get F n (Z,s)
+    -> get F' n' (Z',s')
+    -> get AL' n a
+    -> ParamRel a Z Z' /\ BlockRel a (F.blockI E Z s n) (F.blockI E' Z' s' n').
+
+Lemma simILabenv_extension' t (r:frel) A (PR:ProofRelation A) (AL AL':list A) E E' F F' L L'
+      (LEN1:length AL' = length F)
+  : indexwise_r t (sim'r r \3/ r) PR AL' E E' F F' AL L L'
+    -> indexwise_proofrel PR E E' F F' AL' AL
+    -> (forall n n', IndexRel (AL' ++ AL) n n' -> n < length F -> n' < length F')
+    -> (forall n n', IndexRel (AL' ++ AL) n n' -> n >= length F -> n' >= length F')
+    -> Image AL' = length F'
+    -> simLabenv t r PR AL L L'
+    -> simLabenv t r PR (AL' ++ AL)
+                (mapi (F.mkBlock E) F ++ L)
+                (mapi (F.mkBlock E') F' ++ L').
+Proof.
+  intros ISIM IP Ilt Ige Img SIML.
+  hnf. split.
+  destruct SIML; dcr; split; eauto with len. split; eauto.
+  econstructor; eauto. eapply tooth_F_mkBlocks.
+  econstructor; eauto. eapply tooth_F_mkBlocks.
+  intros ? ? ? ? ? ? ? ? ? V V' RN GetAL GetFL GetL'.
+  assert (❬AL'❭ = ❬mapi (F.mkBlock E) F❭) by eauto with len.
+  eapply get_app_cases in GetAL. destruct GetAL as [GetAL'|GetAL].
+  - eapply get_app_lt_1 in GetFL; [| rewrite <- H; eauto using get_range].
+    inv_get. destruct x as [Z s]. simpl in *. clear EQ.
+    orewrite (n - n = 0). simpl.
+    exploit Ilt; eauto using get_range.
+    eapply get_app_lt_1 in GetL'; [| rewrite mapi_length; eauto with len ].
+    inv_get. destruct x as [Z' s']; simpl in *; clear EQ.
+    split; eauto.
+    intros.
+    exploit (ArgLengthMatchI); eauto; dcr. eapply IP; eauto.
+    exploit (omap_length _ _ _ _ _ H2).
+    exploit (omap_length _ _ _ _ _ H3).
+    pone_step; eauto using get_app, get_mapi; eauto; simpl; try congruence.
+    orewrite (n' - n' = 0); simpl.
+    eapply get_app. eapply mapi_get_1; eauto.
+    simpl. congruence.
+    orewrite (n - n = 0); simpl.
+    orewrite (n' - n' = 0); simpl.
+    eapply ISIM; eauto.
+  - destruct SIML; dcr.
+    eapply get_app_right_ge in GetFL; [ | rewrite <- H; eauto].
+    exploit Ige; eauto; try congruence.
+    eapply get_app_right_ge in GetL'; [ | eauto with len; rewrite mapi_length; eauto].
+    rewrite mapi_length in *.
+    eapply IndexRelDrop in RN; eauto.
+    edestruct H1 as [[? ?] SIM]; eauto. rewrite H; eauto. rewrite Img; eauto.
+    split; eauto.
+    intros.
+    assert (f - n >= ❬mapi (F.mkBlock E) F❭). {
+      exploit (sawtooth_smaller H7 GetFL).
+      rewrite <- H in *. rewrite mapi_length. simpl in *. omega.
+    }
+    assert (f' - n' >= ❬mapi (F.mkBlock E') F'❭). {
+      exploit (sawtooth_smaller H6 GetL').
+      rewrite mapi_length in *.
+      simpl in *. omega.
+    }
+    rewrite (drop_app_gen _ (mapi (F.mkBlock E) F)); eauto.
+    rewrite (drop_app_gen _ (mapi (F.mkBlock E') F')); eauto.
+    repeat rewrite mapi_length. rewrite H in SIM. rewrite Img in SIM.
+    orewrite (f - n - ❬F❭ = f - ❬F❭ - n).
+    orewrite (f' - n' - ❬F'❭ = f' - ❬F'❭ - n').
+    eapply paco3_mon. eapply SIM; eauto. eauto.
+Qed.
+
+Lemma fix_compatible_I t A (PR:ProofRelation A) AL F F' E E' L L' AL'
+(LEN2:length AL' = length F)
+  : (forall r, simLabenv t r PR (AL' ++ AL) (mapi (F.mkBlock E) F ++ L)
+                     (mapi (F.mkBlock E') F' ++ L')
+            -> indexwise_r t (sim'r r) PR AL' E E' F F' AL L L')
+    -> indexwise_proofrel PR E E' F F' AL' AL
+    -> (forall n n', IndexRel (AL' ++ AL) n n' -> n < length F -> n' < length F')
+    -> (forall n n', IndexRel (AL' ++ AL) n n' -> n >= length F -> n' >= length F')
+    -> Image AL' = length F'
+    -> forall r, simLabenv t r PR AL L L'
+           -> indexwise_r t (sim'r r) PR AL' E E' F F' AL L L'.
+Proof.
+  intros ISIM IP Ilt Ige Img r SIML; pcofix CIH.
+  eapply ISIM; eauto.
+  hnf. split.
+  destruct SIML; dcr; split; eauto with len. split.
+  econstructor; eauto. eapply tooth_F_mkBlocks.
+  econstructor; eauto. eapply tooth_F_mkBlocks.
+  eapply simILabenv_extension'; eauto using simILabenv_mon, indexwise_r_mon.
+Qed.
+
+Lemma simILabenv_extension t A (PR:ProofRelation A) (AL AL':list A) E E' F F' L L'
+      (LEN1:length AL' = length F)
+  : (forall r, simLabenv t r PR (AL' ++ AL) (mapi (F.mkBlock E) F ++ L)
+                     (mapi (F.mkBlock E') F' ++ L')
+          -> indexwise_r t (sim'r r) PR AL' E E' F F' AL L L')
+    -> indexwise_proofrel PR E E' F F' AL' AL
+    -> (forall n n', IndexRel (AL' ++ AL) n n' -> n < length F -> n' < length F')
+    -> (forall n n', IndexRel (AL' ++ AL) n n' -> n >= length F -> n' >= length F')
+    -> Image AL' = length F'
+    -> forall r, simLabenv t r PR AL L L'
+           -> simLabenv t r PR (AL' ++ AL)
+                       (mapi (F.mkBlock E) F ++ L)
+                       (mapi (F.mkBlock E') F' ++ L').
+Proof.
+  intros. eapply simILabenv_extension'; eauto.
+  eapply indexwise_r_mon.
+  eapply fix_compatible_I; eauto. eauto.
+Qed.
+
+Lemma renILabenv_extension_len t A (PR:ProofRelation A) (AL AL':list A) E E' F F' L L'
+      (LEN1:length AL' = length F) (LEN2:length F = length F')
+      (IDX:forall AL n n', IndexRel AL n n' = (n = n'))
+  : (forall r, simLabenv t r PR (AL' ++ AL) (mapi (F.mkBlock E) F ++ L)
+                     (mapi (F.mkBlock E') F' ++ L')
+          -> indexwise_r t (sim'r r) PR AL' E E' F F' AL L L')
+    -> indexwise_proofrel PR E E' F F' AL' AL
+    -> Image AL' = length F'
+    -> forall r, simLabenv t r PR AL L L'
+           -> simLabenv t r PR (AL' ++ AL)
+                       (mapi (F.mkBlock E) F ++ L)
+                       (mapi (F.mkBlock E') F' ++ L').
+Proof.
+  assert (forall n n', IndexRel (AL' ++ AL) n n' -> n < length F -> n' < length F').
+  intros. rewrite IDX in H. subst; omega.
+  assert (forall n n', IndexRel (AL' ++ AL) n n' -> n >= length F -> n' >= length F').
+  intros. rewrite IDX in H0. subst; omega.
+  intros. eapply simILabenv_extension'; eauto.
+  eapply indexwise_r_mon.
+  eapply fix_compatible_I; eauto. eauto.
+Qed.
